tried modifying program to mod the uint directly

CCode/fact.c
@@ -1,4 +1,4 @@
-int factorial(int n) {
+unsigned int factorial(unsigned int n) {
 	if (n < 1) {
 		return 1;
 	}
