Proofs/fact.v
@@ -1,12 +1,14 @@
 (* workaround for not having notation *)
 From iris.heap_lang Require proofmode notation.
+Require compcert.lib.Integers.
 Module iris.
 
+Import compcert.lib.Integers.
 Import proofmode notation.
 
-Definition factI : heap_lang.expr :=
+Definition factI : heap_lang.val :=
   rec: "factI" "n" :=
-    if: "n" < #1 then #1 else "n" * "factI" ("n" - #1)
+    if: "n" < #1 then #1 else ("n" * "factI" ("n" - #1)) `rem` #(Int.max_unsigned)
     .
 
 End iris.
@@ -20,8 +22,8 @@ Require Import Vloc.CCode.fact.
 Definition Vprog : varspecs.  mk_varspecs prog. Defined.
 
 
-Definition nat_relate n vVST vHL :=
-  (((Int.min_signed <= n <= Int.max_signed)%Z -> (vVST = Vint (Int.repr n))%Z) /\ vHL = LitV (heap_lang.LitInt n%Z)).
+Definition nat_relate vVST vHL :=
+  ((exists n, ((vVST = Vint (Int.repr n))%Z) /\ vHL = LitV (heap_lang.LitInt n%Z))).
 
 (* for simplicity, we're ignoring out of bounds errors here *)
 Fixpoint fact n : nat :=
@@ -33,104 +35,115 @@ Fixpoint fact n : nat :=
 (* here, the refines we had before won't work... *)
 Definition fspec :=
   DECLARE _factorial
-  WITH gv: globals, ctx: ref_id, n : Z
-  PRE [ tint ]
-    PROP((Int.min_signed <= n <= Int.max_signed)%Z)
-    PARAMS(Vint (Int.repr n))
+  WITH gv: globals, ctx: ref_id, n : int
+  PRE [ tuint ]
+    PROP()
+    PARAMS(Vint n)
     GLOBALS()
-    SEP(refines_right ctx (App iris.factI (Val (LitV (LitInt n)))))
-  POST [ tint ] 
-    EX n : Z, EX v' : ival, EX v : val,
-    PROP(nat_relate n v v')
+    SEP(refines_right ctx (App (Val iris.factI) (Val (LitV (LitInt (Int.unsigned n))))))
+  POST [ tuint ] 
+    EX v' : ival, EX v : val,
+    PROP(nat_relate v v')
     RETURN(v)
     SEP((refines_right ctx (ectxi_language.of_val v'))).
 
 Definition Gprog : funspecs := [fspec].
 
-
 Lemma fact_lemma : semax_body Vprog Gprog f_factorial fspec.
 Proof.
   start_function. 
   forward_if (
-    PROP((n >= 1)%Z) 
-    LOCAL(temp _n (Vint (Int.repr n))) 
+    PROP((Int.unsigned n >= 1)%Z) 
+    LOCAL(temp _n (Vint n)) 
     SEP(refines_right ctx
-       (BinOp MultOp (Val (LitV (LitInt n)))
-          (App
-             (Val
-                (RecV "factI" "n"
-                   (If (BinOp LtOp (Var "n") (Val (LitV (LitInt 1))))
-                      (Val (LitV (LitInt 1)))
-                      (BinOp MultOp (Var "n")
-                         (App (Var "factI")
-                            (BinOp MinusOp (Var "n") (Val (LitV (LitInt 1)))))))))
-             (Val (LitV (LitInt (n - 1)))))))
+       (BinOp RemOp
+          (BinOp MultOp (Val (LitV (LitInt (Int.unsigned n))))
+             (App
+                (Val
+                   (RecV "factI" "n"
+                      (If (BinOp LtOp (Var "n") (Val (LitV (LitInt 1))))
+                         (Val (LitV (LitInt 1)))
+                         (BinOp RemOp
+                            (BinOp MultOp (Var "n")
+                               (App (Var "factI")
+                                  (BinOp MinusOp (Var "n")
+                                     (Val (LitV (LitInt 1))))))
+                            (Val (LitV (LitInt Int.max_unsigned)))))))
+                (BinOp MinusOp (Val (LitV (LitInt (Int.unsigned n))))
+                   (Val (LitV (LitInt 1))))))
+          (Val (LitV (LitInt Int.max_unsigned)))))
   ).
   (* n is zero or less *)
   {
     (* step hl to right form *)
-    do 5 step_pure_r ctx.
+    do 4 step_pure_r ctx.
     forward.
     simpl.
     replace (Z.pos (1 * 1)) with (Z.pos 1) by lia.
-    Exists 1%Z.
     Exists (LitV (heap_lang.LitInt 1%Z)).
     Exists (Vint (Int.repr 1)).
     entailer!.
     unfold nat_relate.
-    auto.
+    eauto.
   }
   {
     (* step hl through 1 cycle *)
-    do 6 step_pure_r ctx.
+    do 4 step_pure_r ctx.
     forward.
+    unfold iris.factI.
     entailer!.
   }
   Intros.
-  forward_call (gv, add_to_ctx ctx [BinOpRCtx MultOp (Val (LitV (LitInt n)))], (n-1)%Z); try lia.
+  step_pure_r ctx.
+  forward_call (gv, add_to_ctx ctx ([BinOpRCtx MultOp (Val (LitV (LitInt (Int.unsigned n))))] ++ [BinOpLCtx RemOp ((LitV (LitInt Int.max_unsigned)))]), (Int.sub n Int.one)); try lia.
   {
     unfold iris.factI.
-    (* we need to step the rhs once to handle the fact that it didn't recure fully? *)
-    replace (App (heap_lang.Rec _ _ _)) with 
-      (App (Val
-           (RecV "factI" "n"
-              (If (BinOp LtOp (Var "n") (Val (LitV (LitInt 1))))
-                 (Val (LitV (LitInt 1)))
-                 (BinOp MultOp (Var "n")
-                    (App (Var "factI")
-                       (BinOp MinusOp (Var "n") (Val (LitV (LitInt 1)))))))))).
-     2:{
-       (* TODO: figure out how to turn heap_lang.Rec into Val (RecV ... or rewrite the program *)
-       admit.
-     }
-    replace (BinOp _ _ _) with (fill [BinOpRCtx MultOp (Val (LitV (LitInt n)))] (App
-        (Val
-           (RecV "factI" "n"
-              (If (BinOp LtOp (Var "n") (Val (LitV (LitInt 1))))
-                 (Val (LitV (LitInt 1)))
-                 (BinOp MultOp (Var "n")
-                    (App (Var "factI")
-                       (BinOp MinusOp (Var "n") (Val (LitV (LitInt 1)))))))))
-        (Val (LitV (LitInt (n - 1)))))) by by rewrite ? fill_app.
+    replace (BinOp _ _ _) with (
+    fill ([BinOpRCtx MultOp (Val (LitV (LitInt (Int.unsigned n))))] ++ [BinOpLCtx RemOp ((LitV (LitInt Int.max_unsigned)))])
+    (App
+         (Val
+            (RecV "factI" "n"
+               (If (BinOp LtOp (Var "n") (Val (LitV (LitInt 1))))
+                  (Val (LitV (LitInt 1)))
+                  (BinOp RemOp
+                     (BinOp MultOp (Var "n")
+                        (App (Var "factI")
+                           (BinOp MinusOp (Var "n") (Val (LitV (LitInt 1))))))
+                     (Val (LitV (LitInt Int.max_unsigned)))))))
+                     (Val (LitV (LitInt (Int.unsigned n - 1)))))
+    ) by by rewrite ? fill_app.
     rewrite refines_right_add_ctx.
+    rewrite Int.unsigned_sub_borrow.
+    rewrite ? Int.unsigned_repr; try rep_lia.
+    unfold Int.sub_borrow; simpl.
+    rewrite if_false.
+    {
+    rewrite ? Int.unsigned_repr; try rep_lia.
+    rewrite Z.add_0_r.
     cancel.
+  }
+    rewrite ? Int.unsigned_repr; try rep_lia.
   }
   (* extract recursive value *)
   Intros ret.
-  destruct ret as [[rn iret] vret]; simpl; simpl in H1. 
+  destruct ret as [iret vret]; simpl; simpl in H0. 
   rewrite <- refines_right_add_ctx; simpl.
-  unfold nat_relate in H1.
-  destruct H1 as [Hvst Hiris]; subst.
+  unfold nat_relate in H0.
+  destruct H0 as [rn [Hvst Hiris]]; subst.
   step_pure_r ctx.
   forward.
-  - entailer!.
-    (* TODO: how to get bounds? I can try to add it to the implication but then other things break *)
+  entailer!.
+  unfold nat_relate.
+  Exists (LitV (LitInt (Int.unsigned n * rn))).
+  Exists (Vint (Int.mul n (Int.repr rn))).
+  simpl.
+  entailer!.
+  exists (Int.unsigned n * rn)%Z.
+  split.
+  - unfold Int.mul.
+    rewrite Int.unsigned_repr; try rep_lia; auto.
+
     admit.
-  - Exists (n * rn)%Z.
-    unfold nat_relate.
-    Exists (LitV (LitInt (n * rn))).
-    Exists (Vint (Int.repr (n * rn))).
-    simpl.
-    entailer!.
-    (* again, I need bounds to solve this *)
+  - auto.
+  (* again, I need bounds to solve this *)
 Admitted.
